FY/Examples.v
@@ -1,0 +1,53 @@
+From FY Require Export Syntax.
+From FY Require Export Semantics.
+From FY Require Export Logic.
+From Coq Require Import Lia.
+From Coq Require Import Strings.String.
+From Coq Require Import Init.Nat.
+
+Definition W : string := "W".
+Definition X : string := "X".
+Definition Y : string := "Y".
+Definition Z : string := "Z".
+
+Definition fact_in_coq : com :=
+  <{ Z := X;
+     Y := 1;
+     while ~(Z = 0) do
+       Y := Y * Z;
+       Z := Z - 1
+     end }>.
+Print fact_in_coq.
+
+Example ceval_example1:
+  empty_st =[
+     X := 2;
+     if (X <= 1)
+       then Y := 3
+       else Z := 4
+     end
+  ]=> (Z !-> 4 ; X !-> 2).
+Proof.
+  (* We must supply the intermediate state *)
+  apply E_Seq with (X !-> 2).
+  - (* assignment command *)
+    apply E_Ass. reflexivity.
+  - (* if command *)
+    apply E_IfFalse.
+    reflexivity.
+    apply E_Ass. reflexivity.
+Qed.
+
+Example ifexample :
+  {{True}}
+  if X = 0 then Y := 2 else Y := X + 1 end
+  {{X <= Y}}.
+Proof.
+  apply hoare_if.
+  - eapply hoare_consequence_pre.
+    + apply hoare_asgn.
+    + assn_auto'. destruct H. apply eqb_eq' in H0. rewrite H0. lia.
+  - eapply hoare_consequence_pre.
+    + apply hoare_asgn.
+    + assn_auto'.
+Qed.
