FY/State.v
@@ -2,6 +2,7 @@
 (* Map *)
 From FY Require Export Map.
 From FY Require Export Matrix.
+From FY Require Export Qubit.
 
 (* State : (classical_map, density_matrix) *)
 Definition state {m n : nat} := (total_map R, Matrix m n).
